\documentclass[14pt]{article}
%\usepackage[cp866nav]{inputenc}
\usepackage[cp1251]{inputenc}
\usepackage[intlimits,sumlimits]{amsmath}
\usepackage{enumerate,graphicx,dcolumn,amsthm}
\usepackage[english,russian,ukrainian]{babel}

\usepackage{floatflt}

\usepackage{tabularx}
\renewcommand{\tabularxcolumn}[1]{m{#1}}
\usepackage{hhline}
\usepackage{multirow}

 \usepackage[left=20mm,right=20mm,top=20mm,bottom=16mm,bindingoffset=0mm,footskip=6mm,includefoot]{geometry}
\setlength{\parindent}{5mm}
\usepackage[hang,flushmargin]{footmisc}

\usepackage{amssymb}


\numberwithin{equation}{part}



\begin{document}           % End of preamble and beginning of text.
\fontsize{14}{16pt}\selectfont


\renewcommand{\theequation}{\thepart.\arabic{equation}}
\begin{equation*}
    I(V)=I_0\left\{\exp \left[\frac{q(V-IR_s)}{nkT}\right]-1\right\}+\frac{V-IR_s}{R_{sh}}
\end{equation*}

rr

\begin{equation*}
    =A+B\,t+C\,t^2
\end{equation*}

rr

\begin{equation*}
    y =A+B\,x
\end{equation*}

rr

\begin{equation*}
    y =A+B\,x+C\,x^2
\end{equation*}

rr

\begin{eqnarray*}
    I(V) =I_0\exp\left(\frac{V}{nkT}\right)\\
    \Phi_b=\frac{kT}{q}\ln\left(\frac{SA^*\,T^{\,2}}{I_0^{\,2}}\right)
\end{eqnarray*}

rr

\begin{equation*}
    y_{i,new} =0.17\,y_{i-1}+0.66\,y_i+0.17\,y_{i+1}
\end{equation*}

rr

\begin{equation*}
    y_{i,new} =\text{middle}\,(y_{i-1},\,y_i,\,y_{i+1})
\end{equation*}

rr

\begin{equation*}
    y_{i,new} =\frac{y_{i-1}(x_i-x_{i+1})}{(x_{i-1}-x_i)(x_{i-1}-x_{i+1})} +
               \frac{y_{i}(2x_i-x_{i-1}-x_{i+1})}{(x_{i}-x_{i-1})(x_{i}-x_{i+1})}+
               \frac{y_{i+1}(x_i-x_{i-1})}{(x_{i+1}-x_{i-1})(x_{i+1}-x_{i})}
\end{equation*}

rr

\begin{equation*}
    y = A + B\,x+c\,\ln x
\end{equation*}

rr

\begin{eqnarray*}
% \nonumber to remove numbering (before each equation)
  I& =& SA^*T^2\exp(-q\Phi_b/kT)\exp(qV_s/kT) \\
  V&=& V_s +\frac{d}{\varepsilon}\sqrt{\frac{2qN_d\varepsilon}{\varepsilon_0}}
       \left(\sqrt{\Phi_b}-\sqrt{\Phi_b-V_s}\,\right)
\end{eqnarray*}

rr

\begin{equation*}
    I(V)=I_0\left\{\exp \left[\frac{q(V-IR_s)}{nkT}\right]-1\right\}+\frac{V-IR_s}{R_{sh}}-I_{ph}
\end{equation*}

rr

\begin{equation*}
    I(V)=\frac{nkT}{qR_s}LambertW\left\{\frac{qR_s}{nkT}
      \exp\left[\frac{q}{nkT}(V+R_sI_0)\right]  \right\}+\frac{V}{R_{sh}}-I_0
\end{equation*}

rr

\begin{eqnarray*}
% \nonumber to remove numbering (before each equation)
  I(V)&=& \frac{nkT}{qR_s} LambertW\left\{\frac{qR_s\left(I_{SC}-\frac{V_{OC}}{R_{sh}+R_s}\right)}{nkT}
      \exp\left[\frac{q\left(R_sI_{SC}+\frac{R_{sh}V}{R_{sh}+R_s}-V_{OC}\right)}{nkT}\right]\right\}\\
   &+& \frac{V}{R_s}-I_{SC}-\frac{R_{sh}V}{R_s(R_{sh}+R_s)}
\end{eqnarray*}

rr

\begin{equation*}
    I(V)=I_{01}\left\{\exp \left[\frac{q(V-IR_{s1})}{n_1kT}\right]-1\right\}+
         I_{02}\left\{\exp \left[\frac{qV}{n_2kT}\right]-1\right\}
\end{equation*}

rr

\begin{equation*}
    I(V)=I_{01}\left\{\exp \left[\frac{q(V-IR_{s1})}{n_1kT}\right]-1\right\}+
         I_{02}\left\{\exp \left[\frac{q(V-IR_{s2})}{n_2kT}\right]-1\right\}
\end{equation*}

rr

\begin{eqnarray*}
  \Phi_b(T)&= -kT\ln &\left\{A\exp\left[-\frac{1}{kT}\left(\Phi_{b0,1}-\frac{\beta T^2}{\alpha+T}\right)+\frac{\sigma_1^2}{2k^2T^2}\right]\right. \\
   &&+ \left.(1-A)\exp\left[-\frac{1}{kT}\left(\Phi_{b0,2}-\frac{\beta T^2}{\alpha+T}\right)+\frac{\sigma_2^2}{2k^2T^2}\right]\right\}
\end{eqnarray*}

rr

\begin{eqnarray*}
  \Phi_b(T)= \Phi_{b0}(T)-\gamma\left(\frac{V_{bb}}{\eta}\right)^{1/3}-\frac{kT}{q}\ln\left[
   \frac{4C_1\pi kT\gamma}{9q}\left(\frac{\eta}{V_{bb}}\right)^{2/3}\right]
 \\
   \Phi_{b0}(T)=\Phi_{b0}-\frac{\beta T^2}{\alpha+T};\,\,
   V_{bb}= \Phi_{b0}(T)-\frac{kT}{q}\ln\left[\frac{2.5\cdot10^{25}}{N_d}\left(\frac{m^*}{m_0}\right)
     \left(\frac{T}{300}\right)^{3/2}\right];\,\,
   \eta=\frac{\varepsilon_0\varepsilon_s}{qN_d}
\end{eqnarray*}

rr

\begin{equation*}
    I(V)=I_{01}\left\{\exp \left[\frac{q(V-IR_s)}{n_1kT}\right]-1\right\}+I_{02}\left\{\exp \left[\frac{q(V-IR_s)}{n_2kT}\right]-1\right\}+\frac{V-IR_s}{R_{sh}}
\end{equation*}

rr
\begin{eqnarray*}
  I(V)&=&I_{01}\left\{\exp \left[\frac{q(V-IR_s)}{n_1kT}\right]-1\right\}+I_{02}\left\{\exp \left[\frac{q(V-IR_s)}{n_2kT}\right]-1\right\}+ \\
   &&I_{03}\left\{\exp \left[\frac{q(V-IR_s)}{n_3kT}\right]-1\right\}+\frac{V-IR_s}{R_{sh}}
\end{eqnarray*}

rr

\begin{eqnarray*}
  I(V)&=&-I_{ph}+I_{01}\left\{\exp \left[\frac{q(V-IR_s)}{n_1kT}\right]-1\right\}+I_{02}\left\{\exp \left[\frac{q(V-IR_s)}{n_2kT}\right]-1\right\}+ \\
   &&I_{03}\left\{\exp \left[\frac{q(V-IR_s)}{n_3kT}\right]-1\right\}+\frac{V-IR_s}{R_{sh}}
\end{eqnarray*}

rr
\begin{equation*}
    I(V)=-I_{ph}+I_{01}\left\{\exp \left[\frac{q(V-IR_s)}{n_1kT}\right]-1\right\}+I_{02}\left\{\exp \left[\frac{q(V-IR_s)}{n_2kT}\right]-1\right\}+\frac{V-IR_s}{R_{sh}}
\end{equation*}

rr

\begin{equation*}
    I(V)=\frac{V}{R}
\end{equation*}

rr

\begin{equation*}
    I\left(\frac{1}{kT}\right)=I_{01}T^{\,2}\exp\left(-\frac{E_1}{kT}\right)+
       I_{02}T^{\,m}\exp\left(-\frac{E_2}{kT}\right)=I_{TE}+I_{SCLC} \,\, if L>0
\end{equation*}

rr


\begin{eqnarray*}
    I\left(\frac{1}{kT}\right)=I_{01}T^{\,2}\exp\left(-\frac{E_1}{kT}\right)+
       I_{02}T^{\,m}\exp\left(-\frac{E_2}{kT}\right)& \qquad \mbox{if}\quad b\geq0 \\
    I\left(\frac{1}{kT}\right)=\frac{I_{01}T^{\,2}\exp\left(-\frac{E_1}{kT}\right)\times I_{02}T^{\,m}\exp\left(-\frac{E_2}{kT}\right)}
    {I_{01}T^{\,2}\exp\left(-\frac{E_1}{kT}\right)+ I_{02}T^{\,m}\exp\left(-\frac{E_2}{kT}\right)}&\qquad \mbox{if}\quad b<0
\end{eqnarray*}


rr


\begin{eqnarray*}
    I_{rev}&(V)&=I_{01}V^{\,p}+I_{02}\exp\left(\frac{AE_m}{kT}\right)\left[1-\exp\left(-\frac{V}{kT}\right)\right] \\
    E_m&=&\left\{\frac{2qN_d}{\varepsilon_0\varepsilon_s}\left[\Phi_{b0}-\frac{\beta T^2}{\alpha+T}-\frac{kT}{q}\ln\left[\frac{2.5\cdot10^{25}}{N_d}\left(\frac{m^*}{m_0}\right)
     \left(\frac{T}{300}\right)^{3/2}\right]+V\right]\right\}^{1/2}
\end{eqnarray*}


rr


\begin{eqnarray*}
    I_{rev}&(V)&=I_{01}\left(V^{1+T_{01}/T}+bV^{1+T_{02}/T}\right)+I_{02}\exp\left(\frac{AE_m}{kT}\right)\left[1-\exp\left(-\frac{V}{kT}\right)\right] \\
    E_m&=&\left\{\frac{2qN_d}{\varepsilon_0\varepsilon_s}\left[\Phi_{b0}-\frac{\beta T^2}{\alpha+T}-\frac{kT}{q}\ln\left[\frac{2.5\cdot10^{25}}{N_d}\left(\frac{m^*}{m_0}\right)
     \left(\frac{T}{300}\right)^{3/2}\right]+V\right]\right\}^{1/2}
\end{eqnarray*}


rr


\begin{eqnarray*}
    I_{rev}&(V)&=I_{01}V^{\,p_1}+I_{02}V^{\,p_2}+I_{03}\exp\left(\frac{AE_m}{kT}\right)\left[1-\exp\left(-\frac{V}{kT}\right)\right] \\
    E_m&=&\left\{\frac{2qN_d}{\varepsilon_0\varepsilon_s}\left[\Phi_{b0}-\frac{\beta T^2}{\alpha+T}-\frac{kT}{q}\ln\left[\frac{2.5\cdot10^{25}}{N_d}\left(\frac{m^*}{m_0}\right)
     \left(\frac{T}{300}\right)^{3/2}\right]+V\right]\right\}^{1/2}
\end{eqnarray*}


rr


\begin{equation*}
    I(V)=I_0\exp\left(-A\sqrt{B+V}\right)
\end{equation*}

rr


\begin{equation*}
    y(x)=A_1\left(x^{m_1}+A_2x^{m_2}\right)
\end{equation*}

\begin{eqnarray*}
    I_{rev}&(V)&=\left[I_{01}\exp\left(\frac{A_1E_m+B\sqrt{E_m}}{kT}\right)+I_{02}\exp\left(\frac{A_2E_m}{kT}\right)\right]
    \left[1-\exp\left(-\frac{V}{kT}\right)\right] \\
    E_m&=&\left\{\frac{2qN_d}{\varepsilon_0\varepsilon_s}\left[\Phi_{b0}-\frac{\beta T^2}{\alpha+T}-\frac{kT}{q}\ln\left[\frac{2.5\cdot10^{25}}{N_d}\left(\frac{m^*}{m_0}\right)
     \left(\frac{T}{300}\right)^{3/2}\right]+V\right]\right\}^{1/2}
\end{eqnarray*}

ff

\begin{equation*}
    I\left(\frac{1}{kT}\right)=I_{01}T^{\,2}\exp\left(-\frac{E}{kT}\right)+
       I_{02}T^{\,m}A^{300/T}
\end{equation*}

ff

\begin{equation*}
    I\left(\frac{1}{kT}\right)=I_{01}T^{\,2}\exp\left(-\frac{E}{kT}\right)+
       I_{02}T^{\,m}\exp\left[-\left(\frac{T_c}{T}\right)^{\!p}\,\right]
\end{equation*}

ff

\begin{equation*}
    \alpha(T,\omega)=A \,\frac{\omega}{T} \,\frac{B\omega\exp\left(\frac{E}{kT}\right)}{1+(B\omega)^2\exp\left(\frac{2E}{kT}\right)}
\end{equation*}

ff

\begin{equation*}
    \alpha(\omega)=A \,\frac{\omega}{T} \,\frac{B\omega\exp\left(\frac{E}{kT}\right)}{1+(B\omega)^2\exp\left(\frac{2E}{kT}\right)}
\end{equation*}

ff
\pagebreak

$I$--$V$ characteristic is approximated by
\begin{eqnarray*}
I&=&AA^*\,T^2\exp\left(-\frac{\Phi_b}{kT}\right)\exp\left(-\frac{qV_s}{kT}\right)\\
V&=&V_s+\frac{d}{\varepsilon_i}\,\sqrt{\frac{2qN_d\,\varepsilon_s}{\varepsilon_0}}\left(\sqrt{\frac{\Phi_b}{q}}-\sqrt{\frac{\Phi_b}{q}-V_s}\,\right)
\end{eqnarray*}
$A$ is the diode area,
$A^*$ is the effective Richardson constant,
$\Phi_b$ is the barrier height,
$d$ is the thickness of the interfacial insulator laye,
$N_d$ is the semiconductor carrier concentration,
$\varepsilon_0$, $\varepsilon_s$ and $\varepsilon_i$ are the permittivities of free space, semiconductor and insulator layer respectively.

$d/\varepsilon_i$ and $\Phi_b$ are defined by approximation.

Density of interface states $D_{is}$ is defined by
\begin{equation*}
    D_{is}=\frac{\varepsilon_i\varepsilon_0}{q^2d}\,\frac{d(V_{cal}-V_{mea})}{d V_s}
\end{equation*}
$V_{cal}$ and $V_{mea}$ are calculated and measured voltage at equal $I$ value,

\noindent
energy of interface states with respect to the conduction band bottom $(E_c-E_{is})$
\begin{equation*}
    (E_c-E_{is})=(\Phi_b-qV_s)
\end{equation*}
$[\,D_{is}\,]= $eV$^{-1}$cm$^{-2}$, $[\,E_c-E_{is}\,]=$ eV.


ff
\pagebreak

Bohlin used two different Norde's functions (two values of $\gamma$):
\begin{eqnarray}
\label{eqBohlin}
F_1(V)&=&\frac{V}{\gamma_1}-\frac{kT}{q}\ln\left(\frac{I(V)}{AA^*T^2}\right),
\nonumber\\
F_2(V)&=&\frac{V}{\gamma_2}-\frac{kT}{q}\ln\left(\frac{I(V)}{AA^*T^2}\right),\nonumber
\end{eqnarray}
$A$ is the diode area,
$A^*$ is the effective Richardson constant,
$\gamma_1$ and $\gamma_2$ are arbitrary constants greater than the ideality factor $n$.

If $[F_{1,min}, V_{min,1}]$ and $[F_{2,min}, V_{min,2}]$ are the coordinates of minimum points in the plots $F_1(V)$ vs $V$ and $F_2(V)$ vs $V$ respectively;
$I_{min,1}$ and $I_{min,2}$ are the current values at the voltage $V_{min,1}$ and $V_{min,2}$ respectively, then
\begin{eqnarray}
\label{eqBohlinDet}
n&=&\frac{1}{2}\left[\frac{\gamma_1I_{min,2}-\gamma_2I_{min,1}}{I_{min,2}-I_{min,1}}+
\frac{V_{min,1}-V_{min,2}+(\gamma_2-\gamma_1)kT/q}{F_{2,min}-F_{1,min}-V_{min,2}/\gamma_2+V_{min,1}/\gamma_1}\right]
,\nonumber
\\
Rs&=&\frac{kT}{2q}\left[\frac{\gamma_1-n}{I_{min,1}}+\frac{\gamma_2-n}{I_{min,2}}\right]\,,\nonumber
\\
\Phi_b&=&\frac{1}{2}\left[F_{1,min}+\frac{(\gamma_1-n)(qV_{min,1}-\gamma_1kT)}{\gamma_1qn}\,+
F_{2,min}+\frac{(\gamma_2-n)(qV_{min,2}-\gamma_2kT)}{\gamma_2qn}\right],\nonumber
\end{eqnarray}
$R_s$ is the series resistance,
$\Phi_b$ is zero bias Schottky barrier height.

\pagebreak

\begin{eqnarray*}
    I_{rev}\left(\frac{1}{kT}, V\right)&=&qSN_{ss}W \\
    W&=&\frac{qE_m}{8m^*\varepsilon_t}\left(1-\frac{\gamma}{\gamma_1}\right)^{1/2}\exp
    \left\{-\frac{4\sqrt{2m^*}\,\varepsilon_t^{3/2}\left(\gamma_1-\gamma\right)^2}{3qE_m\hbar}
    [\gamma_1+0.5\gamma]\right\}\\
    \gamma_1&=&(1+\gamma^2)^{1/2}\\
    \gamma&=&\frac{a\hbar\omega^2\sqrt{2m^*}}{qE_m\sqrt{\varepsilon_t}}
    \left\{\frac{\exp\left(\frac{\hbar\omega}{kT}\right)+1}{\exp\left(\frac{\hbar\omega}{kT}\right)-1}\right\}\\
    E_m&=&\left\{\frac{2qN_d}{\varepsilon_0\varepsilon_s}\left[\Phi_{b0}-\frac{\beta T^2}{\alpha+T}-\frac{kT}{q}\ln\left(\frac{N_C}{N_d}\right)+V\right]\right\}^{1/2}
\end{eqnarray*}

ff

\begin{eqnarray*}
    I_{rev}\left(\frac{1}{kT}, V\right)&=&qSN_{ss}W\left(E_m,\frac{1}{kT},\varepsilon_t,a,\hbar\omega\right)+\\
    &&S_{eff}SA^*T^2\exp\left(-\frac{\Phi_{b0}-\alpha E_m}{kT/q}\right)\left[1-\exp\left(-\frac{qV}{kT}\right)\right]\\
    E_m&=&\left\{\frac{2qN_d}{\varepsilon_0\varepsilon_s}\left[\Phi_{b0}-\frac{\beta T^2}{\alpha+T}-\frac{kT}{q}\ln\left(\frac{N_C}{N_d}\right)+V\right]\right\}^{1/2}
\end{eqnarray*}

ff

\begin{eqnarray*}
    I_{rev}\left(\frac{1}{kT}\right)&=&S_{eff}SA^*T^2\exp\left(-\frac{\Phi_{b0}-\alpha E_m}{kT/q}\right)\left[1-\exp\left(-\frac{qV}{kT}\right)\right]+I_{02}T^{\,m}A^{300/T}\\
    E_m&=&\left\{\frac{2qN_d}{\varepsilon_0\varepsilon_s}\left[\Phi_{b0}-\frac{\beta T^2}{\alpha+T}-\frac{kT}{q}\ln\left(\frac{N_C}{N_d}\right)+V\right]\right\}^{1/2}
\end{eqnarray*}

ff

\begin{eqnarray*}
    I_{rev}\left(\frac{1}{kT}, V\right)&=&qSN_{ss}W\left(E_m,\frac{1}{kT},\varepsilon_t,a,\hbar\omega\right)+
    I_{0}T^{\,2}\exp\left(-\frac{E}{kT}\right)\\
    E_m&=&\left\{\frac{2qN_d}{\varepsilon_0\varepsilon_s}\left[\Phi_{b0}-\frac{\beta T^2}{\alpha+T}-\frac{kT}{q}\ln\left(\frac{N_C}{N_d}\right)+V\right]\right\}^{1/2}
\end{eqnarray*}

rr

\begin{equation*}
    I(V)=I_0\exp \left[A(V-IR_s)\right]+\frac{V-IR_s}{R_{sh}}
\end{equation*}

rr

\begin{equation*}
    I(V)=I_0\exp \left[A(V-IR_s)\right]+\frac{V-IR_s}{R_{sh}}-I_{ph}
\end{equation*}


rr

\begin{equation*}
    I_{SC}(T,\lambda)=N_{ph}(\lambda)\,\frac{\alpha(T,\lambda)\cdot L_0(T/300)^{\,m}}{1+\alpha(T,\lambda)\cdot L_0(T/300)^{\,m}}
\end{equation*}
where
\begin{equation*}
    N_{ph}=\frac{W_{ph}(1-R)q\beta S \lambda}{h c}
\end{equation*}
\begin{eqnarray*}
    \alpha(T,\lambda)&=&\sum_{i,j=1,2}C_iA_j\left[\frac{(hc/\lambda-E_{g,j}(T)+E_{p,i})^2}{\exp(E_{p,i}/kT)-1}+
       \frac{(hc/\lambda-E_{g,j}(T)-E_{p,i})^2}{1-\exp(-E_{p,i}/kT)}\right]\\
       &&+A_d(hc/\lambda-E_{g,d}(T))^{1/2}
\end{eqnarray*}
  $C_1=5.5$,
  $C_2=4.0$,
  $A_1=3.231\times10^2$cm$^{-1}$eV$^{-2}$,
  $A_2=7.237\times10^3$cm$^{-1}$eV$^{-2}$,
  $A_d=1.052\times10^6$cm$^{-1}$eV$^{-2}$,
  $E_g$ are described be Varshni equation,
  $E_{g,1}(0)=1.169$eV,
  $E_{g,2}(0)=2.5$eV,
  $E_{g,d}(0)=3.2$eV.



rr

\begin{equation*}
    \tau_{g}\left(\frac{1}{kT}\right)=\sqrt{SnSp}\left[\exp\left(\frac{E_t}{kT}\right)+\exp\left(-\frac{E_t}{kT}\right)\right]
\end{equation*}

rr

\begin{equation*}
    \tau_{g}\left(\frac{1}{kT}\right)=2\,\tau_{r}\,T^m\sqrt{S_nS_p}\,\cosh\left(\frac{E_t}{kT}\right)
\end{equation*}
rr

\begin{eqnarray*}
    I_{TAT}(V)&=&I_0(U_d+V)\exp\left(-\frac{4\sqrt{2m^*}E_t^{3/2}}{3q\hbar E}\right)+I_{ph}\\
    E&=&\left\{\frac{qN_d(U_d+V)}{2\varepsilon_0\varepsilon_s}\right\}^{1/2}
\end{eqnarray*}

rr

\begin{eqnarray*}
    I_{TAT}(V)&=&I_0(U_d+V-IR_s)\exp\left(-\frac{4\sqrt{2m^*}E_t^{3/2}}{3q\hbar E}\right)\\
    E&=&\left\{\frac{qN_d(U_d+V-IR_s)}{2\varepsilon_0\varepsilon_s}\right\}^{1/2}
\end{eqnarray*}

rr

\begin{equation*}
   F_b(V)=F_{b,0}-a V-b\sqrt{V}
\end{equation*}

rr

\begin{eqnarray*}
  I(V)&=&\frac{Sqn_i^2}{N_d}\sqrt{\frac{\mu k T}{\tau_n}}\left\{\exp \left[\frac{q(V-IR_s)}{n_1kT}\right]-1\right\}+\\
  &&\frac{Sqn_iW}{2\tau_g}\left\{\exp \left[\frac{q(V-IR_s)}{n_2kT}\right]-1\right\}+ \frac{V-IR_s}{R_{sh}}
\end{eqnarray*}


rr

\begin{eqnarray*}
  I(V)&=&-I_{ph}+\frac{Sqn_i^2}{N_d}\sqrt{\frac{\mu k T}{\tau_n}}\left\{\exp \left[\frac{q(V-IR_s)}{n_1kT}\right]-1\right\}+\\
  &&\frac{Sqn_iW}{2\tau_g}\left\{\exp \left[\frac{q(V-IR_s)}{n_2kT}\right]-1\right\}+ \frac{V-IR_s}{R_{sh}}
\end{eqnarray*}


rr

\begin{equation*}
  \tau=\frac{A(T/300)^{m-0.5}}{(1+BT)^2}
\end{equation*}

see \emph{J. Appl. Phys.} \textbf{110}, 053713 (2011)



\begin{equation*}
  R_{SH}(T)=AT\left[\cosh\left(\frac{E_t}{kT}-U_0\right)+\cosh\left(\frac{qU_s}{kT}-U_0\right)\right]
\end{equation*}

rr

\begin{eqnarray*}
    R_{SH}(T)&=&\frac{R_{disl}R_{met}}{R_{disl}+R_{met}}\\
    R_{disl}&=&AT\left[\cosh\left(\frac{E_t}{kT}\right)+\cosh\left(\frac{qU_s}{kT}\right)\right]\\
    R_{met}&=&R_0\left[1+(T-293)\alpha\right]
\end{eqnarray*}

rr

\begin{equation*}
  y=a_0+a_1x^{m_1}+a_2x^{m_2}
\end{equation*}

\begin{eqnarray*}
    \mu(T)&=&(\mu_n^{-1}+\mu_{disl}^{-1}+\mu_i^{-1}+\mu_{ph}^{-1}+\mu_{pz}^{-1}+\mu_{F}^{-1})^{-1}\\
    \mu_n&=&A_n\\
    \mu_{disl}&=&A_{disl}\,T\\
    \mu_{i}&=&A_{i}\,T^{3/2}\\
    \mu_{ph}&=&A_{ph}\,T^{-3/2}\\
    \mu_{pz}&=&A_{pz}\,T^{-1/2}\\
    \mu_{F}&=&A_{f}\,\exp\left(-\frac{Fb}{kT}\right)
\end{eqnarray*}


rr

\begin{equation*}
    n(T)=n_i(T)+\sum_{i=1}^{i=4}N_{di}[1-f_{FD}(T,E_{di})]-\sum_{j=1}^{j=3}N_{tj}f_{FD}(T,E_{tj})-N_a
\end{equation*}
where
$N_a$ is the acceptor density,
$n_i$ is the intrinsic concentration
\begin{equation*}
    n_i(T)=[N_c(T)N_v(T)]^{0.5}\exp\left[-\frac{E_G(T)}{2kT}\right]\,,
\end{equation*}
$N_{di}$ is the density an $i$th donor,

\noindent
$E_{di}$ is the energy level of an $i$th donor from $E_c$,

\noindent
$N_{tj}$ and $E_{tj}$ are the density and energy level of an $j$th electron trap,

\noindent
$f_{FD}(T,E)$ is the Fermi--Dirac distribution function for donors

\noindent
and electron traps
\begin{equation*}
    f_{FD}(T,E)=\left\{1+\frac{1}{2}\exp\left[\frac{E_F(T)-E}{kT}\right]\right\}^{-1}\,.
\end{equation*}

rr

\begin{equation*}
    n(N_B, T)=1+\frac{n_0T^{m_T}(\lg N_B)^{m_B}}{1+\frac{N_{v,Si}(T)}{N_B}\exp\left(-\frac{E_{ef}}{kT}\right)}
\end{equation*}

\begin{equation*}
    E_{ef}=E_{ef,0}-\frac{E_B T}{\lg N_B}+E_T T
\end{equation*}

$\qquad\qquad$boron concentration $N_B$ ($[N_B]=$cm$^{-3}$) in first column of file,

$\qquad\qquad$ $T$ in second column,
ideality factor $n$ in $N_{fCol}$ column


rr

\begin{equation*}
    n(N_Fe, N_B, T)=1+\frac{n_0T(\lg N_B)^{3}(\lg N_{Fe})^{3}}{1+\frac{N_{v,Si}(T)}{N_B}\exp\left(-\frac{E_{ef}}{kT}\right)}
\end{equation*}

\begin{equation*}
    E_{ef}=E_{ef,0}-\frac{E_B T}{\lg N_B}+E_T T+\frac{E_{Fe}}{\lg N_{Fe}}
\end{equation*}

$\qquad\qquad$iron concentration $N_{Fe}$ must be in first column of file,

$\qquad\qquad$boron concentration $N_B$ in second column of file ($[N_B],\, [N_{Fe}]=$cm$^{-3}$),

$\qquad\qquad$$T$ in third column,
ideality factor $n$ in $N_{fCol}$ column


rr

\begin{equation*}
    n(T)=1+\frac{n_0T^{m_T}}{1+\gamma N_{v,Si}(T)\exp\left(-\frac{E_{eff}}{kT}\right)}
\end{equation*}



rr

\begin{equation*}
    y=a_0+a_1\,x+a_2\,x^2+\ldots+a_n\,x^n
\end{equation*}


rr

\begin{equation*}
    y_{i,new} =\frac{y_i+y_{i-1}+\ldots+y_{i-N_p+1}}{N_p}
\end{equation*}


rr

- Data are divided in sub--ranges with $N_p$ points;

- For each sub--range $\{x_i\}$ and $\{y_i\}$ are processed independently:

i) $z_{max}$ and $z_{min}$ ($z=(x, y)$) are deleted;

ii) $z_{i,new} =M_{ean}+[(P_{os}-N_{eg})|D_{tot}|]\frac{1}{(N_p-2)^2}$,

where $M_{ean}=\frac{1}{N_p-2}\cdot\sum z_i$;
$P_{os}$ ($N_{eg}$) --- number of $z_i>M_{ean}$ ($z_i<M_{ean}$);

$D_{tot}=\sum_{i \in P_{os}} (z_i-M_{ean})$.




\begin{equation*}
    S_{i} =y_{i}+b_i(x-x_{i})+c_i(x-x_{i})^2+d_i(x-x_{i})^3\,;
\end{equation*}
\begin{equation*}
    x_{i}\leqslant x\leqslant x_{i+1}, \: i=\overline{0,(n-1)}\,;
\end{equation*}
\begin{equation*}
    S_{i}(x_i)=S_{i+1}(x_i)=y_i;\;S_{i}^{\:\prime}(x_i)=S_{i+1}^{\:\prime}(x_i);\;
    S_{i}^{\:\prime\prime}(x_i)=S_{i+1}^{\:\prime\prime}(x_i)
\end{equation*}

rr


\begin{equation*}
    y_{i,new} =a_0\,y_i+a_1\,y_{i-1}+\ldots+b_0\,y_{i-1,new}+b_1\,y_{i-2,new}\ldots\,;
\end{equation*}

\hspace{1cm}number of terms depends on number of poles,

\hspace{1cm}coefficient values depend on number of poles and cutoff frequency.


rr

\begin{eqnarray*}
  y_{i,new} &=& (1-\alpha)\,y_i+\alpha\,y_{i-1,new}\,; \\
   \alpha&=&\exp(-2\pi\,f_{co})
\end{eqnarray*}


rr

\begin{eqnarray*}
  y_{i,new} &=& (1-\alpha)^4\,y_i+4\alpha\,y_{i-1,new}-6\alpha^2\,y_{i-2,new}+ \\
   && +4\alpha^3\,y_{i-2,new}-\alpha^4\,y_{i-3,new}\,; \\
    \alpha&=&\exp(-2\pi\,f_{co})
\end{eqnarray*}


rr


\begin{equation*}
    y_{i,new} = \sum_{k=0}^{N_{FO}-1}a_k\,y_{i-k}\,;
\end{equation*}
\begin{equation*}
    a_k=\frac{\sin\left[2\pi\,f_{co}\left(k-\frac{N_{FO}-1}{2}\right)\right]}{\pi\left(k-\frac{N_{FO}-1}{2}\right)}\,;
\end{equation*}

\hspace{5cm} $N_{FO}$ --- filter order

rr

\begin{equation*}
    y_{i,new} = \sum_{k=0}^{N_{FO}-1}a_k\,y_{i-k}\,;
\end{equation*}
\begin{equation*}
    a_k=\frac{\sin\left[2\pi\,f_{co}\left(k-\frac{N_{FO}-1}{2}\right)\right]}{\pi\left(k-\frac{N_{FO}-1}{2}\right)}
    \left[0.42-0.5\cos\left(\frac{2\pi k}{N_{FO}-1}\right)+0.08\cos\left(\frac{4\pi k}{N_{FO}-1}\right)\right]\,;
\end{equation*}
%\hspace{5cm}
 $N_{FO}$ --- filter order

rr

\begin{equation*}
    y_{i,new} = \sum_{k=0}^{N_{FO}-1}a_k\,y_{i-k}\,;
\end{equation*}
\begin{equation*}
    a_k=\frac{\sin\left[2\pi\,f_{co}\left(k-\frac{N_{FO}-1}{2}\right)\right]}{\pi\left(k-\frac{N_{FO}-1}{2}\right)}
    \left[0.53836-0.46164\cos\left(\frac{2\pi k}{N_{FO}-1}\right)\right]\,;
\end{equation*}
\hspace{1.5cm}
 $N_{FO}$ --- filter order

rr

\begin{equation*}
    y_{i,new} = \sum_{k=0}^{N_{FO}-1}a_k\,y_{i-k}\,;
\end{equation*}
\begin{equation*}
    a_k=\frac{\sin\left[2\pi\,f_{co}\left(k-\frac{N_{FO}-1}{2}\right)\right]}{\pi\left(k-\frac{N_{FO}-1}{2}\right)}
    \cdot0.5\cdot\left[1-\cos\left(\frac{2\pi k}{N_{FO}-1}\right)\right]\,;
\end{equation*}
\hspace{2.5cm}
 $N_{FO}$ --- filter order

rr

\begin{equation*}
    y_{i,new} = \sum_{k=0}^{N_{FO}-1}a_k\,y_{i-k}\,;
\end{equation*}
\begin{equation*}
    a_k=
   \left\{
   \begin{aligned}
   &\frac{2k}{N_{FO}-1}\,, \quad\text{if}\quad \:k\leqslant\frac{N_{FO}-1}{2} \\
   &2-\frac{2k}{N_{FO}-1}\,, \quad\text{else}
    \end{aligned}
     \right.\,;
\end{equation*}
\hspace{5cm}
 $N_{FO}$ --- filter order

rr

\begin{equation*}
    y_{i,new} = \sum_{k=0}^{N_{FO}-1}a_k\,y_{i-k}\,;
\end{equation*}
\begin{equation*}
    a_k=
   \left\{
   \begin{aligned}
   &\frac{\sin\left[2\pi\,f_{co}\left(k-\frac{N_{FO}-1}{2}\right)\right]}{\pi\left(k-\frac{N_{FO}-1}{2}\right)}
    \cdot\frac{\cosh\left[N_{FO}\cdot\text{arccosh}\left(|\beta|\right)\right]}
              {\cosh\left[N_{FO}\cdot\text{arccosh}\left(\alpha\right)\right]}\,,
              \quad\text{if}\: |\beta|>1 \\
   &\frac{\sin\left[2\pi\,f_{co}\left(k-\frac{N_{FO}-1}{2}\right)\right]}{\pi\left(k-\frac{N_{FO}-1}{2}\right)}
    \cdot\frac{\cosh\left[N_{FO}\cdot\text{arccosh}\left(\beta\right)\right]}
              {\cosh\left[N_{FO}\cdot\text{arccosh}\left(\alpha\right)\right]}\,,
               \quad\text{else}
    \end{aligned}
     \right.\,;
\end{equation*}
\begin{equation*}
    \beta = \alpha\cdot\cos\left(\frac{\pi k}{N_{FO}}\right)\,;
    \qquad \alpha=\cosh\left[\frac{\text{arccosh}\left(10^{A/20}\right)}{N_{FO}}\right]
\end{equation*}
\hspace{1cm}
 $N_{FO}$ --- filter order;
 $A$ --- minor lobe level, $[A]=$~dB.

 rr

\begin{equation*}
    y_{i,new} = \sum_{k=0}^{N_{FO}-1}a_k\,y_{i-k}\,;
\end{equation*}
\begin{equation*}
    a_k=\frac{\cos\left[2\pi\,f_{co}\left(k-\frac{N_{FO}-1}{2}\right)\right]}{\pi\left(k-\frac{N_{FO}-1}{2}\right)}\,;
\end{equation*}

\hspace{5cm} $N_{FO}$ --- filter order

rr

\begin{eqnarray*}
  V&=&(I+I_{ph}+I_{0,1})R_{sh,1}-\\
  &&-\frac{n_1kT}{q}LambertW\left\{\frac{q}{n_1kT}I_{0,1}R_{sh,1}
  \exp\left[\frac{q}{n_1kT}R_{sh,1}\left(I+I_{ph}+I_{0,1}\right)\right]\right\}+\\
  &&+\frac{n_2kT}{q}LambertW\left\{\frac{q}{n_2kT}I_{0,2}R_{sh,2}
  \exp\left[-\frac{q}{n_2kT}R_{sh,2}\left(I-I_{0,2}\right)\right]\right\}+\\
  &&+\left(I-I_{0,2}\right)R_{sh,2}+IR_s
\end{eqnarray*}

\begin{eqnarray*}
% \nonumber to remove numbering (before each equation)
  V &=& IR_s+\frac{n_1kT}{q}\cdot g\left(x_1\right)-\frac{n_2kT}{q}\cdot g\left(x_2\right)- \\
  &&-\frac{n_1kT}{q}\cdot\log\left[\frac{q}{n_1kT}I_{0,1}R_{sh,1}\right]
  +\frac{n_2kT}{q}\cdot\log\left[\frac{q}{n_2kT}I_{0,2}R_{sh,2}\right]
\end{eqnarray*}

\begin{eqnarray*}
% \nonumber to remove numbering (before each equation)
  x_1 &=& \log\left(\frac{q}{n_1kT}I_{0,1}R_{sh,1}\right)+\frac{q}{n_1kT}R_{sh,1}\left(I+I_{ph}+I_{0,1}\right) \\
  x_2&=& \log\left(\frac{q}{n_2kT}I_{0,2}R_{sh,2}\right)+\frac{q}{n_2kT}R_{sh,2}\left(I-I_{0,2}\right)
\end{eqnarray*}

\begin{equation*}
  g(x)=\log\left(LambertW\left(\exp(x)\right)\right)
\end{equation*}

\begin{equation*}
  g_{n+1}(x)=g_n(x)-\frac{2\,\left[g_n+\exp\left(g_n\right)-x\right]\cdot\left[1+\exp\left(g_n\right)\right]}
  {2\,\left[1+\exp\left(g_n\right)\right]^2-\left[g_n+\exp\left(g_n\right)-x\right]\cdot\exp\left(g_n\right)}
\end{equation*}

\begin{equation*}
    g_0(x)=
   \left\{
   \begin{aligned}
   &x\,,\;\;\qquad \qquad\qquad\qquad\quad\text{if}\quad x\leqslant-e \\
   &-e+\frac{1+e}{2e}\cdot(x+e)\,,\quad\text{if}\quad -e<x<e \\
    &\log(x)\,,\;\; \quad\qquad\qquad\qquad\text{if}\quad x\geqslant e          
    \end{aligned}
     \right.\,;
\end{equation*}

rr

\begin{equation*}
  y=\sum_{i=1}^{N}A_i\frac{\exp\left[-\frac{\left(x-x_{0,i}\right)^2}{2\sigma_i^2}\right]}{\sigma_i\sqrt{2\pi}}
\end{equation*}

\end{document} 